fsti prop

proofs/fstar/extraction-edited/Libcrux.Kem.Kyber.Kyber768.fsti
@@ -3,6 +3,65 @@ module Libcrux.Kem.Kyber.Kyber768
 open Core
 open FStar.Mul
 
+let v_ETA1: usize = sz 2
+
+let v_ETA1_RANDOMNESS_SIZE: usize = v_ETA1 *! sz 64
+
+let v_ETA2: usize = sz 2
+
+let v_ETA2_RANDOMNESS_SIZE: usize = v_ETA2 *! sz 64
+
+let v_RANK_768_: usize = sz 3
+
+let v_CPA_PKE_SECRET_KEY_SIZE_768_: usize =
+  ((v_RANK_768_ *! Libcrux.Kem.Kyber.Constants.v_COEFFICIENTS_IN_RING_ELEMENT <: usize) *!
+    Libcrux.Kem.Kyber.Constants.v_BITS_PER_COEFFICIENT
+    <:
+    usize) /!
+  sz 8
+
+let v_RANKED_BYTES_PER_RING_ELEMENT_768_: usize =
+  (v_RANK_768_ *! Libcrux.Kem.Kyber.Constants.v_BITS_PER_RING_ELEMENT <: usize) /! sz 8
+
+let v_T_AS_NTT_ENCODED_SIZE_768_: usize =
+  ((v_RANK_768_ *! Libcrux.Kem.Kyber.Constants.v_COEFFICIENTS_IN_RING_ELEMENT <: usize) *!
+    Libcrux.Kem.Kyber.Constants.v_BITS_PER_COEFFICIENT
+    <:
+    usize) /!
+  sz 8
+
+let v_CPA_PKE_PUBLIC_KEY_SIZE_768_: usize = v_T_AS_NTT_ENCODED_SIZE_768_ +! sz 32
+
+let v_SECRET_KEY_SIZE_768_: usize =
+  ((v_CPA_PKE_SECRET_KEY_SIZE_768_ +! v_CPA_PKE_PUBLIC_KEY_SIZE_768_ <: usize) +!
+    Libcrux.Kem.Kyber.Constants.v_H_DIGEST_SIZE
+    <:
+    usize) +!
+  Libcrux.Kem.Kyber.Constants.v_SHARED_SECRET_SIZE
+
+let v_VECTOR_U_COMPRESSION_FACTOR_768_: usize = sz 10
+
+let v_C1_BLOCK_SIZE_768_: usize =
+  (Libcrux.Kem.Kyber.Constants.v_COEFFICIENTS_IN_RING_ELEMENT *! v_VECTOR_U_COMPRESSION_FACTOR_768_
+    <:
+    usize) /!
+  sz 8
+
+let v_C1_SIZE_768_: usize = v_C1_BLOCK_SIZE_768_ *! v_RANK_768_
+
+let v_VECTOR_V_COMPRESSION_FACTOR_768_: usize = sz 4
+
+let v_C2_SIZE_768_: usize =
+  (Libcrux.Kem.Kyber.Constants.v_COEFFICIENTS_IN_RING_ELEMENT *! v_VECTOR_V_COMPRESSION_FACTOR_768_
+    <:
+    usize) /!
+  sz 8
+
+let v_CPA_PKE_CIPHERTEXT_SIZE_768_: usize = v_C1_SIZE_768_ +! v_C2_SIZE_768_
+
+let v_IMPLICIT_REJECTION_HASH_INPUT_SIZE: usize =
+  Libcrux.Kem.Kyber.Constants.v_SHARED_SECRET_SIZE +! v_CPA_PKE_CIPHERTEXT_SIZE_768_
+
 unfold
 let t_Kyber768Ciphertext = Libcrux.Kem.Kyber.Types.t_KyberCiphertext (sz 1088)
 
