proofs/fstar/extraction-edited/Libcrux.Kem.Kyber.Ind_cpa.fst
@@ -40,20 +40,6 @@ let into_padded_array (v_LEN: usize) (slice: t_Slice u8) =
 unfold let acc_t v_K = (u8 & t_Array u8 (sz 33) & t_Array Libcrux.Kem.Kyber.Arithmetic.t_PolynomialRingElement v_K)
 unfold let inv_t v_K = acc_t v_K -> usize -> Type
 
-val sample_vector_cbd (#p:Spec.Kyber.params)
-      (v_K v_ETA2_RANDOMNESS_SIZE v_ETA2: usize)
-      (prf_input: t_Array u8 (sz 33))
-      (domain_separator: u8)
-    : Pure (t_Array u8 (sz 33) & u8 & t_Array Libcrux.Kem.Kyber.Arithmetic.t_PolynomialRingElement v_K)
-      (requires v domain_separator <= v v_K /\ v_K <=. sz 4 /\
-                v_K = p.v_RANK /\ v_ETA2 = p.v_ETA2 /\
-                v_ETA2_RANDOMNESS_SIZE = Spec.Kyber.v_ETA2_RANDOMNESS_SIZE p)
-      (ensures (fun (prf,ds,x) -> v ds == v domain_separator + v v_K /\
-                Seq.slice prf 0 32 == Seq.slice prf_input 0 32 /\
-                Libcrux.Kem.Kyber.Arithmetic.to_spec_vector #p x ==
-                Spec.Kyber.sample_vector_cbd #p (Seq.slice prf_input 0 32) (sz (v domain_separator))))
-
-
 let sample_vector_cbd (#p:Spec.Kyber.params)
       (v_K v_ETA2_RANDOMNESS_SIZE v_ETA2: usize)
       (prf_input: t_Array u8 (sz 33)) domain_separator = 
@@ -104,16 +90,6 @@ let sample_vector_cbd (#p:Spec.Kyber.params)
   prf_input, domain_separator, hax_temp_output
   <:
   (t_Array u8 (sz 33) & u8 & t_Array Libcrux.Kem.Kyber.Arithmetic.t_PolynomialRingElement v_K)
-
-val sample_vector_cbd_then_ntt (#p:Spec.Kyber.params)
-      (v_K v_ETA v_ETA_RANDOMNESS_SIZE: usize)
-      (prf_input: t_Array u8 (sz 33))
-      (domain_separator: u8{v domain_separator <= v v_K /\ v_K <=. sz 4})
-    : Pure (t_Array Libcrux.Kem.Kyber.Arithmetic.t_PolynomialRingElement v_K & u8) 
-      (requires (v_K == p.v_RANK /\ v_ETA == p.v_ETA1 /\ v_ETA_RANDOMNESS_SIZE == Spec.Kyber.v_ETA1_RANDOMNESS_SIZE p))
-      (ensures (fun (x,ds) -> v ds == v domain_separator + v v_K /\
-                Libcrux.Kem.Kyber.Arithmetic.to_spec_vector #p x ==
-                Spec.Kyber.sample_vector_cbd_then_ntt #p (Seq.slice prf_input 0 32) (sz (v domain_separator))))
 
 let sample_vector_cbd_then_ntt (#p:Spec.Kyber.params)
       (v_K v_ETA v_ETA_RANDOMNESS_SIZE: usize)
@@ -172,17 +148,6 @@ let sample_vector_cbd_then_ntt (#p:Spec.Kyber.params)
   <:
   (t_Array Libcrux.Kem.Kyber.Arithmetic.t_PolynomialRingElement v_K & u8)
 
-val compress_then_serialize_u (#p:Spec.Kyber.params)
-      (v_K v_OUT_LEN v_COMPRESSION_FACTOR v_BLOCK_LEN: usize)
-      (input: t_Array Libcrux.Kem.Kyber.Arithmetic.t_PolynomialRingElement v_K)
-    : Pure (t_Array u8 v_OUT_LEN)
-      (requires (v_K == p.v_RANK /\ v_OUT_LEN == Spec.Kyber.v_C1_SIZE p /\
-                 v_COMPRESSION_FACTOR == p.v_VECTOR_U_COMPRESSION_FACTOR /\
-                 v_BLOCK_LEN = Spec.Kyber.v_C1_BLOCK_SIZE p))
-      (ensures (fun res -> 
-        res == Spec.Kyber.compress_then_encode_u p 
-               (Libcrux.Kem.Kyber.Arithmetic.to_spec_vector #p input)))
-
 let compress_then_serialize_u (#p:Spec.Kyber.params)
       (v_K v_OUT_LEN v_COMPRESSION_FACTOR v_BLOCK_LEN: usize)
       (input: t_Array Libcrux.Kem.Kyber.Arithmetic.t_PolynomialRingElement v_K) =
@@ -235,18 +200,6 @@ let compress_then_serialize_u (#p:Spec.Kyber.params)
   out
 
 #push-options "--split_queries always"
-val deserialize_then_decompress_u (#p:Spec.Kyber.params)
-      (v_K v_CIPHERTEXT_SIZE v_VECTOR_U_ENCODED_SIZE v_U_COMPRESSION_FACTOR: usize)
-      (ciphertext: t_Array u8 v_CIPHERTEXT_SIZE)
-    : Pure (t_Array Libcrux.Kem.Kyber.Arithmetic.t_PolynomialRingElement v_K) 
-      (requires v_K == p.v_RANK /\
-                v_CIPHERTEXT_SIZE == Spec.Kyber.v_CPA_PKE_CIPHERTEXT_SIZE p /\
-                v_VECTOR_U_ENCODED_SIZE == Spec.Kyber.v_C1_SIZE p /\
-                v_U_COMPRESSION_FACTOR == p.v_VECTOR_U_COMPRESSION_FACTOR)
-      (ensures fun res ->
-        Libcrux.Kem.Kyber.Arithmetic.to_spec_vector #p res ==
-        Spec.Kyber.(vector_ntt (decode_then_decompress_u p (Seq.slice ciphertext 0 (v (Spec.Kyber.v_C1_SIZE p))))))
-
 let deserialize_then_decompress_u (#p:Spec.Kyber.params)
       (v_K v_CIPHERTEXT_SIZE v_VECTOR_U_ENCODED_SIZE v_U_COMPRESSION_FACTOR: usize)
       (ciphertext: t_Array u8 v_CIPHERTEXT_SIZE) =
@@ -296,16 +249,6 @@ let deserialize_then_decompress_u (#p:Spec.Kyber.params)
   admit(); //P-F
   u_as_ntt
 
-val deserialize_public_key (#p:Spec.Kyber.params) 
-    (v_K v_T_AS_NTT_ENCODED_SIZE: usize) (public_key: t_Slice u8)
-    : Pure (t_Array Libcrux.Kem.Kyber.Arithmetic.t_PolynomialRingElement v_K)
-      (requires v_K == p.v_RANK /\
-                length public_key == Spec.Kyber.v_CPA_PKE_PUBLIC_KEY_SIZE p /\
-                v_T_AS_NTT_ENCODED_SIZE == Spec.Kyber.v_T_AS_NTT_ENCODED_SIZE p)
-      (ensures fun res -> 
-        Libcrux.Kem.Kyber.Arithmetic.to_spec_vector res ==
-        Spec.Kyber.vector_decode_12 #p (slice public_key (sz 0) v_T_AS_NTT_ENCODED_SIZE))
-   
 let deserialize_public_key (#p:Spec.Kyber.params) 
     (v_K v_T_AS_NTT_ENCODED_SIZE: usize) (public_key: t_Slice u8) =
   let tt_as_ntt:t_Array Libcrux.Kem.Kyber.Arithmetic.t_PolynomialRingElement v_K =
@@ -338,14 +281,6 @@ let deserialize_public_key (#p:Spec.Kyber.params)
   admit(); //P-F
   tt_as_ntt 
 
-val deserialize_secret_key (#p:Spec.Kyber.params) (v_K: usize) (secret_key: t_Slice u8)
-    : Pure (t_Array Libcrux.Kem.Kyber.Arithmetic.t_PolynomialRingElement v_K)
-      (requires v_K == p.v_RANK /\
-                length secret_key == Spec.Kyber.v_CPA_PKE_SECRET_KEY_SIZE p)
-      (ensures fun res ->
-         Libcrux.Kem.Kyber.Arithmetic.to_spec_vector #p res ==
-         Spec.Kyber.vector_decode_12 #p secret_key)
-    
 let deserialize_secret_key (#p:Spec.Kyber.params) (v_K: usize) (secret_key: t_Slice u8) =
   let secret_as_ntt:t_Array Libcrux.Kem.Kyber.Arithmetic.t_PolynomialRingElement v_K =
     Rust_primitives.Hax.repeat Libcrux.Kem.Kyber.Arithmetic.impl__PolynomialRingElement__ZERO v_K
@@ -499,15 +434,6 @@ let encrypt #p
   ciphertext
 #pop-options
 
-val serialize_secret_key (#p:Spec.Kyber.params)
-      (v_K v_OUT_LEN: usize)
-      (key: t_Array Libcrux.Kem.Kyber.Arithmetic.t_PolynomialRingElement v_K)
-    : Pure (t_Array u8 v_OUT_LEN)
-      (requires (v_K == p.v_RANK /\ v_OUT_LEN == Spec.Kyber.v_CPA_PKE_SECRET_KEY_SIZE p))
-      (ensures (fun res -> 
-        res == Spec.Kyber.vector_encode_12 #p 
-          (Libcrux.Kem.Kyber.Arithmetic.to_spec_vector #p key)))
-      
 let serialize_secret_key (#p:Spec.Kyber.params)
       (v_K v_OUT_LEN: usize)
       (key: t_Array Libcrux.Kem.Kyber.Arithmetic.t_PolynomialRingElement v_K) =
@@ -564,18 +490,6 @@ let serialize_secret_key (#p:Spec.Kyber.params)
   admit(); //P-F
   out
 
-val serialize_public_key (#p:Spec.Kyber.params)
-      (v_K v_RANKED_BYTES_PER_RING_ELEMENT v_PUBLIC_KEY_SIZE: usize)
-      (tt_as_ntt: t_Array Libcrux.Kem.Kyber.Arithmetic.t_PolynomialRingElement v_K)
-      (seed_for_a: t_Slice u8)
-      : Pure (t_Array u8 v_PUBLIC_KEY_SIZE)
-        (requires (v_K == p.v_RANK /\
-                   v_RANKED_BYTES_PER_RING_ELEMENT == Spec.Kyber.v_RANKED_BYTES_PER_RING_ELEMENT p /\
-                   v_PUBLIC_KEY_SIZE == Spec.Kyber.v_CPA_PKE_PUBLIC_KEY_SIZE p /\
-                   length seed_for_a == sz 32))
-        (ensures (fun res -> res == Seq.append (Spec.Kyber.vector_encode_12 
-                              (Libcrux.Kem.Kyber.Arithmetic.to_spec_vector #p tt_as_ntt))
-                            seed_for_a))
 
 let serialize_public_key (#p:Spec.Kyber.params)
       (v_K v_RANKED_BYTES_PER_RING_ELEMENT v_PUBLIC_KEY_SIZE: usize)
