proofs/fstar/extraction-edited/Libcrux.Kem.Kyber.Ind_cpa.fsti
@@ -8,6 +8,72 @@ val into_padded_array (v_LEN: usize) (slice: t_Slice u8) :
     (requires (length slice <=. v_LEN))
     (ensures (fun res ->  Seq.slice res 0 (Seq.length slice) == slice))
 
+val sample_vector_cbd (#p:Spec.Kyber.params)
+      (v_K v_ETA2_RANDOMNESS_SIZE v_ETA2: usize)
+      (prf_input: t_Array u8 (sz 33))
+      (domain_separator: u8)
+    : Pure (t_Array u8 (sz 33) & u8 & t_Array Libcrux.Kem.Kyber.Arithmetic.t_PolynomialRingElement v_K)
+      (requires v domain_separator <= v v_K /\ v_K <=. sz 4 /\
+                v_K = p.v_RANK /\ v_ETA2 = p.v_ETA2 /\
+                v_ETA2_RANDOMNESS_SIZE = Spec.Kyber.v_ETA2_RANDOMNESS_SIZE p)
+      (ensures (fun (prf,ds,x) -> v ds == v domain_separator + v v_K /\
+                Seq.slice prf 0 32 == Seq.slice prf_input 0 32 /\
+                Libcrux.Kem.Kyber.Arithmetic.to_spec_vector #p x ==
+                Spec.Kyber.sample_vector_cbd #p (Seq.slice prf_input 0 32) (sz (v domain_separator))))
+
+
+val sample_vector_cbd_then_ntt (#p:Spec.Kyber.params)
+      (v_K v_ETA v_ETA_RANDOMNESS_SIZE: usize)
+      (prf_input: t_Array u8 (sz 33))
+      (domain_separator: u8{v domain_separator <= v v_K /\ v_K <=. sz 4})
+    : Pure (t_Array Libcrux.Kem.Kyber.Arithmetic.t_PolynomialRingElement v_K & u8) 
+      (requires (v_K == p.v_RANK /\ v_ETA == p.v_ETA1 /\ v_ETA_RANDOMNESS_SIZE == Spec.Kyber.v_ETA1_RANDOMNESS_SIZE p))
+      (ensures (fun (x,ds) -> v ds == v domain_separator + v v_K /\
+                Libcrux.Kem.Kyber.Arithmetic.to_spec_vector #p x ==
+                Spec.Kyber.sample_vector_cbd_then_ntt #p (Seq.slice prf_input 0 32) (sz (v domain_separator))))
+
+val compress_then_serialize_u (#p:Spec.Kyber.params)
+      (v_K v_OUT_LEN v_COMPRESSION_FACTOR v_BLOCK_LEN: usize)
+      (input: t_Array Libcrux.Kem.Kyber.Arithmetic.t_PolynomialRingElement v_K)
+    : Pure (t_Array u8 v_OUT_LEN)
+      (requires (v_K == p.v_RANK /\ v_OUT_LEN == Spec.Kyber.v_C1_SIZE p /\
+                 v_COMPRESSION_FACTOR == p.v_VECTOR_U_COMPRESSION_FACTOR /\
+                 v_BLOCK_LEN = Spec.Kyber.v_C1_BLOCK_SIZE p))
+      (ensures (fun res -> 
+        res == Spec.Kyber.compress_then_encode_u p 
+               (Libcrux.Kem.Kyber.Arithmetic.to_spec_vector #p input)))
+
+val deserialize_then_decompress_u (#p:Spec.Kyber.params)
+      (v_K v_CIPHERTEXT_SIZE v_VECTOR_U_ENCODED_SIZE v_U_COMPRESSION_FACTOR: usize)
+      (ciphertext: t_Array u8 v_CIPHERTEXT_SIZE)
+    : Pure (t_Array Libcrux.Kem.Kyber.Arithmetic.t_PolynomialRingElement v_K) 
+      (requires v_K == p.v_RANK /\
+                v_CIPHERTEXT_SIZE == Spec.Kyber.v_CPA_PKE_CIPHERTEXT_SIZE p /\
+                v_VECTOR_U_ENCODED_SIZE == Spec.Kyber.v_C1_SIZE p /\
+                v_U_COMPRESSION_FACTOR == p.v_VECTOR_U_COMPRESSION_FACTOR)
+      (ensures fun res ->
+        Libcrux.Kem.Kyber.Arithmetic.to_spec_vector #p res ==
+        Spec.Kyber.(vector_ntt (decode_then_decompress_u p (Seq.slice ciphertext 0 (v (Spec.Kyber.v_C1_SIZE p))))))
+
+val deserialize_public_key (#p:Spec.Kyber.params) 
+    (v_K v_T_AS_NTT_ENCODED_SIZE: usize) (public_key: t_Slice u8)
+    : Pure (t_Array Libcrux.Kem.Kyber.Arithmetic.t_PolynomialRingElement v_K)
+      (requires v_K == p.v_RANK /\
+                length public_key == Spec.Kyber.v_CPA_PKE_PUBLIC_KEY_SIZE p /\
+                v_T_AS_NTT_ENCODED_SIZE == Spec.Kyber.v_T_AS_NTT_ENCODED_SIZE p)
+      (ensures fun res -> 
+        Libcrux.Kem.Kyber.Arithmetic.to_spec_vector res ==
+        Spec.Kyber.vector_decode_12 #p (slice public_key (sz 0) v_T_AS_NTT_ENCODED_SIZE))
+   
+val deserialize_secret_key (#p:Spec.Kyber.params) (v_K: usize) (secret_key: t_Slice u8)
+    : Pure (t_Array Libcrux.Kem.Kyber.Arithmetic.t_PolynomialRingElement v_K)
+      (requires v_K == p.v_RANK /\
+                length secret_key == Spec.Kyber.v_CPA_PKE_SECRET_KEY_SIZE p)
+      (ensures fun res ->
+         Libcrux.Kem.Kyber.Arithmetic.to_spec_vector #p res ==
+         Spec.Kyber.vector_decode_12 #p secret_key)
+    
+
 val decrypt (#p:Spec.Kyber.params)
       (v_K v_CIPHERTEXT_SIZE v_VECTOR_U_ENCODED_SIZE v_U_COMPRESSION_FACTOR v_V_COMPRESSION_FACTOR:
           usize)
@@ -47,6 +113,27 @@ val encrypt (#p:Spec.Kyber.params)
                  v_C2_LEN == Spec.Kyber.v_C2_SIZE p))
       (ensures (fun ct -> ct == Spec.Kyber.ind_cpa_encrypt p public_key message randomness))
                
+val serialize_secret_key (#p:Spec.Kyber.params)
+      (v_K v_OUT_LEN: usize)
+      (key: t_Array Libcrux.Kem.Kyber.Arithmetic.t_PolynomialRingElement v_K)
+    : Pure (t_Array u8 v_OUT_LEN)
+      (requires (v_K == p.v_RANK /\ v_OUT_LEN == Spec.Kyber.v_CPA_PKE_SECRET_KEY_SIZE p))
+      (ensures (fun res -> 
+        res == Spec.Kyber.vector_encode_12 #p 
+          (Libcrux.Kem.Kyber.Arithmetic.to_spec_vector #p key)))
+      
+val serialize_public_key (#p:Spec.Kyber.params)
+      (v_K v_RANKED_BYTES_PER_RING_ELEMENT v_PUBLIC_KEY_SIZE: usize)
+      (tt_as_ntt: t_Array Libcrux.Kem.Kyber.Arithmetic.t_PolynomialRingElement v_K)
+      (seed_for_a: t_Slice u8)
+      : Pure (t_Array u8 v_PUBLIC_KEY_SIZE)
+        (requires (v_K == p.v_RANK /\
+                   v_RANKED_BYTES_PER_RING_ELEMENT == Spec.Kyber.v_RANKED_BYTES_PER_RING_ELEMENT p /\
+                   v_PUBLIC_KEY_SIZE == Spec.Kyber.v_CPA_PKE_PUBLIC_KEY_SIZE p /\
+                   length seed_for_a == sz 32))
+        (ensures (fun res -> res == Seq.append (Spec.Kyber.vector_encode_12 
+                              (Libcrux.Kem.Kyber.Arithmetic.to_spec_vector #p tt_as_ntt))
+                            seed_for_a))
 
 val generate_keypair (#p:Spec.Kyber.params)
       (v_K v_PRIVATE_KEY_SIZE v_PUBLIC_KEY_SIZE v_RANKED_BYTES_PER_RING_ELEMENT v_ETA1 v_ETA1_RANDOMNESS_SIZE:
